@prefix rdf: <http://www.w3.org/1999/02/22-rdf-syntax-ns#> .
@prefix owl: <http://www.w3.org/2002/07/owl#> .
@prefix rdfs: <http://www.w3.org/2000/01/rdf-schema#> .
@prefix :     <http://colin.maudry.com/ontologies/dgfr#> .
@prefix dcterms: <http://purl.org/dc/terms/> .
@prefix foaf: <http://xmlns.com/foaf/0.1/> .
@prefix xsd: <http://www.w3.org/2001/XMLSchema#> . 
@prefix frbr: <http://purl.org/vocab/frbr/core#> .
@prefix cc: <http://creativecommons.org/ns#> .
@prefix vann: <http://purl.org/vocab/vann/> .
@prefix dcat: <http://www.w3.org/ns/dcat#> .
@prefix prov: <http://www.w3.org/ns/prov#> .
@prefix schema: <http://schema.org/> .

#Author: Colin Maudry
#Contact: colin@maudry.com


#The following data.gouv.fr properties are mapped with Dublin Core or DCAT properties during the conversion:

# For datasets and resources
# id			> dct:identifier
# created_at 	> dct:created
# last_modified	> dct:modified

#For datasets
# frequency 	> dct:accrualPeriodicity
# organization 	> dct:rightsHolder
# supplier 		> dct:publisher
# url 			> dcat:landingPage
# tags			> dcat:keyword (not implemented yet)

#For resources
# url			> dcat:downloadUrl 
# mime			> dcat:mediaType
# size 			> dcat:byteSize

<http://colin.maudry.com/ontologies/dgfr#>
	a owl:Ontology ;
	dcterms:title "Data.gouv.fr (DGFR) ontology" ;
	dcterms:creator <http://colin.maudry/rdf/colin-maudry#me> ;
	dcterms:created "2014-12-12"^^xsd:date ;
	dcterms:modified "2014-12-12"^^xsd:date ;
	dcterms:description "The DGFR ontology defines the terms required to describe the datasets published or referenced on data.gouv.fr, when DCAT and Dublin Core are not enough."@en ;
	dcterms:description "L'ontologie DGFR définit les termes nécessaires à la description des jeux de données publiés ou référencés sur data.gouv.fr, lorsque DCAT et Dublin Core ne suffisent pas."@fr ;
	cc:license <http://unlicense.org> ;
	vann:preferredNamespaceUri <http://colin.maudry.com/ontologies/dgfr#>;
    vann:preferredNamespacePrefix "dgfr";
	rdfs:seeAlso <http://data.gouv.fr> .

	<http://colin.maudry/rdf/colin-maudry#me> foaf:name "Colin Maudry" ;
		foaf:mbox  <mailto:colin@maudry.com>  . 

#For dcat:Dataset

	:private a rdf:Property ;
		rdfs:isDefinedBy : ;
		rdfs:range xsd:boolean ;
		rdfs:label "Private" ;
		rdfs:comment "Defines whether the dataset is private (not public) or not."@en ;
		rdfs:comment "Détermine si le jeu de données est privé (non public) ou non."@fr ;
		rdfs:domain dcat:Dataset .
	
	:featured a rdf:Property ;
		rdfs:isDefinedBy : ;
		rdfs:range xsd:boolean ;
		rdfs:label "Featured" ;
		rdfs:comment "Defines whether the dataset is shown on the portal front page or not."@en ;
		rdfs:comment "Détermine si le jeu de données est visible sur la page d'accueil du portail, ou non."@fr ;
		rdfs:domain dcat:Dataset .
	
	:views a rdf:Property ;
		rdfs:isDefinedBy : ;
		rdfs:range xsd:integer ;
		rdfs:label "Views" ;
		rdfs:comment "The number of times the page of the dataset bas been viewed."@en ;
		rdfs:comment "Le nombre de fois que la page du jeu de données a été vue."@fr ;
		rdfs:domain dcat:Dataset, foaf:Organization .
	
	:hits a rdf:Property ;
		rdfs:isDefinedBy : ;
		rdfs:range xsd:integer ;
		rdfs:label "Hits" ;
		rdfs:comment "The number of times the page of the dataset bas been viewed. But different from views."@en ;
		rdfs:comment "Le nombre de fois que la page du jeu de données a été vue. Mais différent des views."@fr ;
		rdfs:domain dcat:Dataset, foaf:Organization .
	
	:visits a rdf:Property ;
		rdfs:isDefinedBy : ;
		rdfs:range xsd:integer ;
		rdfs:label "Visits" ;
		rdfs:comment "The number of times the page of the dataset bas been visited."@en ;
		rdfs:comment "Le nombre de fois que la page du jeu de données a été visitée."@fr ;
		rdfs:domain dcat:Dataset, foaf:Organization .
	
	:reuses a rdf:Property ;
		rdfs:isDefinedBy : ;
		rdfs:range xsd:integer ;
		rdfs:label "Reuses" ;
		rdfs:comment "The number of reuses that have been created from the data of the dataset and published on the same page. For an organization, the number of reuses created using its datasets."@en ;
		rdfs:comment "Le nombre de réutilisations qui ont été créées à partir des données du jeu de données et publiés sur la même page. Pour une organisation, le nombre de réutilisations créées à partir de ses jeux de données."@fr ;
		rdfs:domain dcat:Dataset, foaf:Organization .	
		
	:followers a rdf:Property ;
		rdfs:isDefinedBy : ;
		rdfs:range xsd:integer ;
		rdfs:label "Followers" ;
		rdfs:comment "The number of users who subscribed to be informed when the dataset is updated."@en ;
		rdfs:comment "Le nombre d'utilisateurs qui se sont abonnés pour être informés lorsque le jeu de données est mis à jour."@fr ;
		rdfs:domain dcat:Dataset, foaf:Organization .

	:issues a rdf:Property ;
		rdfs:isDefinedBy : ;
		rdfs:range xsd:integer ;
		rdfs:label "Issues" ;
		rdfs:comment "The number of issues that have been reported about the dataset (wrong or missing data)."@en ;
		rdfs:comment "Le nombre d'anomalies qui ont été signalées pour le jeu de données (données erronées ou manquantes)."@fr ;
		rdfs:domain dcat:Dataset .

	:uniqueVisitors a rdf:Property ;
		rdfs:isDefinedBy : ;
		rdfs:range xsd:integer ;
		rdfs:label "Unique visitors" ;
		rdfs:comment "The number of unique visitors who viewed the page of the dataset."@en ;
		rdfs:comment "Le nombre de visiteurs uniques qui se sont rendus sur la page du jeu de données."@fr ;
		rdfs:domain dcat:Dataset, foaf:Organization .	
		
	:slug a rdf:Property ;
		rdfs:isDefinedBy : ;
		rdfs:range xsd:string ;
		rdfs:label "Slug" ;
		rdfs:comment "A URL-friendly version of the title."@en ;
		rdfs:comment "Une version du titre simplifiée pour pouvoir être inséré dans une URL."@fr ;
		rdfs:domain dcat:Dataset, foaf:Organization, :Reuse .	

	:distributions a rdf:Property ;
		rdfs:isDefinedBy : ;
		rdfs:range xsd:integer ;
		rdfs:label "Distributions" ;
		rdfs:comment "The number of distributions that this dataset contains."@en ;
		rdfs:comment "Le nombre de distributions cotenues dans le jeu de données."@fr ;
		rdfs:domain dcat:Dataset .	
		
#For dcat:Distribution

	:type a rdf:Property ;
		rdfs:isDefinedBy : ;
		rdfs:range xsd:string ;
		rdfs:label "Type";
		rdfs:comment "The type of resource (file, remote file, API, etc.)"@en ;
		rdfs:comment "Le type de ressource (fichier, fichier distant, API, etc.)"@fr ;
		rdfs:domain dcat:Distribution . 
	
	:format a rdf:Property ;
		rdfs:isDefinedBy : ;
		rdfs:range xsd:string ;
		rdfs:label "Format" ;
		rdfs:comment "Defines the format of a resource/dcat:Distribution. Used until proper resources of type dct:MediaTypeOrExtent are found."@en ;
		rdfs:comment "Détermine le format d'une ressource/dcat:Distribution. Propriété utilisée jusqu'à ce que l'on trouve des ressources de type dct:MediaTypeOrExtent."@fr ;
		rdfs:domain dcat:Distribution .
	
	:checksumType a rdf:Property ;
		rdfs:isDefinedBy : ;
		rdfs:range xsd:string ;
		rdfs:label "Checksum type" ;
		rdfs:comment "The type of checksum of the resource."@en ;
		rdfs:comment "Le type de somme de contrôle de la ressource."@fr ;
		rdfs:domain dcat:Distribution .

	:checksumValue a rdf:Property ;
		rdfs:isDefinedBy : ;
		rdfs:range xsd:string ;
		rdfs:label "Checksum value" ;
		rdfs:comment "The checksum of the resource."@en ;
		rdfs:comment "La somme de contrôle de la ressource."@fr ;
		rdfs:domain dcat:Distribution .
		
	:downloads a rdf:Property ;
		rdfs:isDefinedBy : ;
		rdfs:range xsd:integer ;
		rdfs:label "Downloads" ;
		rdfs:comment "The number of times the resource was downloaded."@en ;
		rdfs:comment "Le nombre de fois que la ressource a été téléchargée."@fr ;
		rdfs:domain dcat:Distribution .
		
	:dataset a rdf:Property ;
		rdfs:isDefinedBy : ;
		rdfs:range dcat:Dataset ;
		rdfs:label "Dataset" ;
		rdfs:comment "A dataset in which this distribution is included."@en ;
		rdfs:comment "Un jeu de données dans lequel cette ressource est incluse"@fr ;
		rdfs:domain dcat:Distribution .		

#For dgfr:Reuse

	:Reuse rdfs:subClassOf foaf:Document ;
		rdfs:isDefinedBy : ;
		rdfs:label "Reuse" ;
		rdfs:comment "A creative work derived from the data of one or more dataset"@en ;
		rdfs:comment "Une réalisation créée à partir des données d'un ou plusieurs jeux de données"@fr .
	
	:datasets a rdf:Property ;
		rdfs:isDefinedBy : ;
		rdfs:label "Datasets" ;
		rdfs:comment "The number of datasets used to make the reuse"@en ;
		rdfs:comment "Le nombre de jeux de données utilisés pour réaliser la réutilisation"@fr ;
		rdfs:range xsd:integer ;
		rdfs:domain :Reuse, foaf:Organization .
	
	:localUrl rdfs:subPropertyOf schema:url ;
		rdfs:isDefinedBy : ;
		rdfs:label "Remote URL" ;
		rdfs:comment "The URL where a reuse is registered and described on the platform."@en ;
		rdfs:comment "L'URL à laquelle une réutilisation est référencée et décrite sur la plateforme."@fr ;
		rdfs:domain :Reuse .

#For foaf:Organization

	:members a rdf:Property ;
		rdfs:isDefinedBy : ;
		rdfs:label "Members" ;
		rdfs:comment "The number of people that are members of this organization"@en ;
		rdfs:comment "Le nombre de personne qui sont membres de cette organisation"@fr ;
		rdfs:range xsd:integer ;
		rdfs:domain foaf:Organization .
	
	:hasMadeReuses a rdf:Property ;
		rdfs:isDefinedBy : ;
		rdfs:label "Has made reuses" ;
		rdfs:comment "The number of reuses produced and published by this organization"@en ;
		rdfs:comment "Le nombre de réutilisations produites et publiées par cette organisation"@fr ;
		rdfs:range xsd:integer ;
		rdfs:domain foaf:Organization .
		 
	:publicService a rdf:Property ;
		rdfs:isDefinedBy : ;
		rdfs:range xsd:boolean ;
		rdfs:label "Public service" ;
		rdfs:comment "Defines whether the organization is entrusted a mission of public service."@en ;
		rdfs:comment "Détermine si l'organisation est chargée d'une mission de service publique, ou non."@fr ;
		rdfs:domain foaf:Organization .		
	
	:published a rdf:Property ;
		rdfs:isDefinedBy : ;
		owl:inverseOf dcterms:publisher ;
		rdfs:range dcat:Dataset, :Reuse ;
		rdfs:label "Published" ;
		rdfs:comment "A resource that was published by the agent (person or organization)."@en ;
		rdfs:comment "Une entité publiée par un agent (personne ou organisation)"@fr ;
		rdfs:domain foaf:Agent .

:datasets a rdf:Property ;
		rdfs:comment "The number of datasets published "@en ;
		rdfs:range xsd:integer ;
		rdfs:label "Datasets" ;
		rdfs:domain foaf:Agent ;
		rdfs:comment "Le nombre de jeux de données utilisés pour réaliser la réutilisation"@fr .

#For ranking purposes

	:pointsValue a rdf:Property ;
		rdfs:isDefinedBy : ;
		rdfs:range xsd:integer ;
		rdfs:label "Points value" ;
		rdfs:domain rdf:Property ;
		rdfs:comment "The value in points that each unit is worth" .
	
	:popularityPoints a rdf:Property ;
		rdfs:isDefinedBy : ;
		rdfs:domain foaf:Organization, dcat:Dataset, dcat:Distribution, :Reuse ;
		rdfs:range xsd:integer ;
		rdfs:label "Popularity points" ;
		rdfs:comment "For a given object, the number of points related to popularity (downloads, followers)"@en .
	
	:sumPopularityPoints a rdf:Property ;
		rdfs:isDefinedBy : ;
		rdfs:domain foaf:Organization, dcat:Dataset ;
		rdfs:range xsd:integer ;
		rdfs:label "Sum of popularity points" ;
		rdfs:comment "For a given object, the sum of the points calculated at its level plus the points calculated at the level of dependant objects. For instance, a datasets holds the sum of points at its level and at the level of the related distributions."@en .


#Availability

:responseStatusCode a rdf:Property ;
		rdfs:range xsd:string ;
		rdfs:isDefinedBy : ;
		rdfs:comment "The HTTP response code returned by the server when downloading the resource."@en ;
		rdfs:comment "Le code HTTP renvoyé par le serveur lors d'une tentative de téléchargement de la distribution."@fr ;
		rdfs:label "Response status code" ;
		rdfs:domain dcat:Distribution .

:responseTime a rdf:Property ;
		rdfs:range xsd:decimal ;
		rdfs:isDefinedBy : ;
		rdfs:comment "The time, in seconds, for the server that hosts the distribution (file), to respond to a request. This is not the download time."@en ;
		rdfs:comment "Le temps, en seconde, que met le serveur hébergeant la distribution (fichier) pour répondre à une requête. Ce n'est pas le temps téléchargement."@fr ;
		rdfs:label "Response time (seconds)" ;
		rdfs:domain dcat:Distribution .

:available a rdf:Property ;
		rdfs:range xsd:boolean ;
		rdfs:isDefinedBy : ;
		rdfs:comment "Whether the distribution (file) can actually be downloaded or if the server returns an error."@en ;
		rdfs:comment "Si la distribution (fichier) peut véritablement être téléchargée, ou si le serveur renvoie une erreur."@fr ;
		rdfs:label "Available" ;
		rdfs:domain dcat:Distribution .

:availabilityCheckedOn a rdf:Property ;
		rdfs:range xsd:dateTime ;
		rdfs:isDefinedBy : ;
		rdfs:comment "The date and time when the distribution (file) had its availability checked for the last time."@en ;
		rdfs:comment "La date et l'heure auxquelles la disponibilité de la distribution (fichier) a été vérifée pour la dernière fois."@fr ;
		rdfs:label "Availability checked on" ;
		rdfs:domain dcat:Distribution .

:availableDistributions a rdf:Property ;
		rdfs:isDefinedBy : ;
		rdfs:comment "The number of distributions (files) that are actually available."@en ;
		rdfs:range xsd:integer ;
		rdfs:label "Available distributions" ;
		rdfs:domain foaf:Agent , dcat:Dataset ;
		rdfs:comment "Le nombre de distributions (fichiers) qui sont véritablement disponibles."@fr .

:unavailableDistributions a rdf:Property ;
		rdfs:isDefinedBy : ;
		rdfs:comment "The number of distributions (files) for which the hosting server returns an error."@en ;
		rdfs:range xsd:integer ;
		rdfs:label "Unavailable distributions" ;
		rdfs:domain foaf:Agent , dcat:Dataset ;
		rdfs:comment "Le nombre de distributions (fichiers) pour les lesquels le serveur qui les hébérge renvoie une erreur."@fr .

		
